Iris/Iris/Tests/HeapLang/Notation.lean
@@ -13,36 +13,39 @@ open Iris.HeapLang
 
 section test
 
-variable (v : Val)
-/-- info: hl((#1 + (#1 + v(v)))) : Exp -/
+variable (v : Val) (e : Exp)
+/-- info: hl((#1 + (#1 + v(&v)))) : Exp -/
 #guard_msgs in
-#check hl(#1 + #1 + {.val v})
+#check hl(#1 + #1 + &(.ofVal v))
 /--
-info: Exp.binop BinOp.plus (Exp.val (Val.lit (@OfNat.ofNat BaseLit (nat_lit 1) (@instOfNatBaseLit (nat_lit 1)))))
-  (Exp.binop BinOp.plus (Exp.val (Val.lit (@OfNat.ofNat BaseLit (nat_lit 1) (@instOfNatBaseLit (nat_lit 1)))))
-    (Exp.val v)) : Exp
+info: Exp.binop BinOp.plus
+  (@ProgramLogic.ToVal.ofVal Exp Val instToVal (Val.lit ↑(@OfNat.ofNat Int (nat_lit 1) (@instOfNat (nat_lit 1)))))
+  (Exp.binop BinOp.plus
+    (@ProgramLogic.ToVal.ofVal Exp Val instToVal (Val.lit ↑(@OfNat.ofNat Int (nat_lit 1) (@instOfNat (nat_lit 1)))))
+    (@ProgramLogic.ToVal.ofVal Exp Val instToVal v)) : Exp
 -/
 #guard_msgs in
 set_option pp.explicit true in
-#check hl(#1 + #1 + {.val v})
-/-- info: hl((#1 + (#1 + v(v)))) : Exp -/
+#check hl(#1 + #1 + &(.ofVal v))
+/-- info: hl((#1 + (#1 + v(&v)))) : Exp -/
 #guard_msgs in
-#check hl(#1 + (#1 + v(v)))
+#check hl(#1 + (#1 + v(&v)))
 
-/-- info: hl(((#1 + #1) + v(v))) : Exp -/
+/-- info: hl(((#1 + #1) + v(&v))) : Exp -/
 #guard_msgs in
-#check hl((#1 + #1) + v(v))
+#check hl((#1 + #1) + &v)
 
-/-- info: hl((#1 = (v + v(v)))) : Exp -/
+/-- info: hl((#1 = (v + (v(&v) + &e)))) : Exp -/
 #guard_msgs in
-#check hl(#1 = v + v(v))
+#check hl(#1 = v + &v + &e)
 /--
-info: Exp.binop BinOp.eq (Exp.val (Val.lit (@OfNat.ofNat BaseLit (nat_lit 1) (@instOfNatBaseLit (nat_lit 1)))))
-  (Exp.binop BinOp.plus (Exp.var "v") (Exp.val v)) : Exp
+info: Exp.binop BinOp.eq
+  (@ProgramLogic.ToVal.ofVal Exp Val instToVal (Val.lit ↑(@OfNat.ofNat Int (nat_lit 1) (@instOfNat (nat_lit 1)))))
+  (Exp.binop BinOp.plus (Exp.var "v") (@ProgramLogic.ToVal.ofVal Exp Val instToVal v)) : Exp
 -/
 #guard_msgs in
 set_option pp.explicit true in
-#check hl(#1 = v + v(v))
+#check hl(#1 = v + v(&v))
 
 /-- info: hl((λ x y z, #1)) : Exp -/
 #guard_msgs in
@@ -55,7 +58,8 @@ set_option pp.explicit true in
 /--
 info: Exp.rec_ Binder.anon (Binder.named "x")
   (Exp.rec_ Binder.anon (Binder.named "y")
-    (Exp.val (Val.lit (@OfNat.ofNat BaseLit (nat_lit 1) (@instOfNatBaseLit (nat_lit 1)))))) : Exp
+    (@ProgramLogic.ToVal.ofVal Exp Val instToVal
+      (Val.lit ↑(@OfNat.ofNat Int (nat_lit 1) (@instOfNat (nat_lit 1)))))) : Exp
 -/
 #guard_msgs in
 set_option pp.explicit true in
@@ -67,7 +71,7 @@ set_option pp.explicit true in
 
 /--
 info: (Exp.rec_ (Binder.named "f") (Binder.named "x") (Exp.var "x")).app
-  (Exp.val (Val.lit (@OfNat.ofNat BaseLit (nat_lit 1) (@instOfNatBaseLit (nat_lit 1))))) : Exp
+  (@ProgramLogic.ToVal.ofVal Exp Val instToVal (Val.lit ↑(@OfNat.ofNat Int (nat_lit 1) (@instOfNat (nat_lit 1))))) : Exp
 -/
 #guard_msgs in
 set_option pp.explicit true in
@@ -83,20 +87,36 @@ info: Exp.rec_ Binder.anon (Binder.named "x")
     ((Exp.rec_ Binder.anon (Binder.named "z")
           ((Exp.rec_ Binder.anon Binder.anon
                 (Exp.binop BinOp.plus (Exp.var "x") (Exp.binop BinOp.plus (Exp.var "y") (Exp.var "z")))).app
-            (Exp.val (Val.lit (@OfNat.ofNat BaseLit (nat_lit 2) (@instOfNatBaseLit (nat_lit 2))))))).app
-      (Exp.val (Val.lit (@OfNat.ofNat BaseLit (nat_lit 1) (@instOfNatBaseLit (nat_lit 1))))))) : Exp
+            (@ProgramLogic.ToVal.ofVal Exp Val instToVal
+              (Val.lit ↑(@OfNat.ofNat Int (nat_lit 2) (@instOfNat (nat_lit 2))))))).app
+      (@ProgramLogic.ToVal.ofVal Exp Val instToVal
+        (Val.lit ↑(@OfNat.ofNat Int (nat_lit 1) (@instOfNat (nat_lit 1))))))) : Exp
 -/
 #guard_msgs in
 set_option pp.explicit true in
 #check hl(λ x y, let z := #1; #2; x + y + z)
 
+variable (f x : Binder) in
+/-- info: hl((λ &x y, (rec &f &x := y))) : Exp -/
+#guard_msgs in
+#check hl(λ &x y, rec &f &x := y)
+
+variable (f x : Binder) in
+/--
+info: Exp.rec_ Binder.anon x (Exp.rec_ Binder.anon (Binder.named "y") (Exp.rec_ f x (Exp.var "y"))) : Exp
+-/
+#guard_msgs in
+set_option pp.explicit true in
+#check hl(λ &x y, rec &f &x := y)
+
+
 /--
 info: hl((λ x y,
-      ((((#1 + (#2 +ₗ (#3 - (#4 * (#5 / (#6 % #7)))))) & #8) | (#9 ^ (#10 <<< (#11 >>> #12)))) ≤
+      ((((#1 + (#2 +ₗ (#3 - (#4 * (#5 / (#6 % #7)))))) &&& #8) ||| (#9 ^^^ (#10 <<< (#11 >>> #12)))) ≤
           (#13 ≤ (#14 < (#15 = (#16 + ((-#17) + (~#18))))))))) : Exp
 -/
 #guard_msgs in
-#check hl(λ x y, #1 + #2 +ₗ #3 - #4 * #5 / #6 % #7 & #8 | #9 ^ #10 <<< #11 >>> #12 <= #13 ≤ #14 < #15 = #16 + (-#17) + (~#18))
+#check hl(λ x y, #1 + #2 +ₗ #3 - #4 * #5 / #6 % #7 &&& #8 ||| #9 ^^^ #10 <<< #11 >>> #12 <= #13 ≤ #14 < #15 = #16 + (-#17) + (~#18))
 
 /--
 info: Exp.rec_ Binder.anon (Binder.named "x")
@@ -104,43 +124,66 @@ info: Exp.rec_ Binder.anon (Binder.named "x")
     (Exp.binop BinOp.le
       (Exp.binop BinOp.or
         (Exp.binop BinOp.and
-          (Exp.binop BinOp.plus (Exp.val (Val.lit (@OfNat.ofNat BaseLit (nat_lit 1) (@instOfNatBaseLit (nat_lit 1)))))
+          (Exp.binop BinOp.plus
+            (@ProgramLogic.ToVal.ofVal Exp Val instToVal
+              (Val.lit ↑(@OfNat.ofNat Int (nat_lit 1) (@instOfNat (nat_lit 1)))))
             (Exp.binop BinOp.offset
-              (Exp.val (Val.lit (@OfNat.ofNat BaseLit (nat_lit 2) (@instOfNatBaseLit (nat_lit 2)))))
+              (@ProgramLogic.ToVal.ofVal Exp Val instToVal
+                (Val.lit ↑(@OfNat.ofNat Int (nat_lit 2) (@instOfNat (nat_lit 2)))))
               (Exp.binop BinOp.minus
-                (Exp.val (Val.lit (@OfNat.ofNat BaseLit (nat_lit 3) (@instOfNatBaseLit (nat_lit 3)))))
+                (@ProgramLogic.ToVal.ofVal Exp Val instToVal
+                  (Val.lit ↑(@OfNat.ofNat Int (nat_lit 3) (@instOfNat (nat_lit 3)))))
                 (Exp.binop BinOp.mult
-                  (Exp.val (Val.lit (@OfNat.ofNat BaseLit (nat_lit 4) (@instOfNatBaseLit (nat_lit 4)))))
+                  (@ProgramLogic.ToVal.ofVal Exp Val instToVal
+                    (Val.lit ↑(@OfNat.ofNat Int (nat_lit 4) (@instOfNat (nat_lit 4)))))
                   (Exp.binop BinOp.tdiv
-                    (Exp.val (Val.lit (@OfNat.ofNat BaseLit (nat_lit 5) (@instOfNatBaseLit (nat_lit 5)))))
+                    (@ProgramLogic.ToVal.ofVal Exp Val instToVal
+                      (Val.lit ↑(@OfNat.ofNat Int (nat_lit 5) (@instOfNat (nat_lit 5)))))
                     (Exp.binop BinOp.tmod
-                      (Exp.val (Val.lit (@OfNat.ofNat BaseLit (nat_lit 6) (@instOfNatBaseLit (nat_lit 6)))))
-                      (Exp.val (Val.lit (@OfNat.ofNat BaseLit (nat_lit 7) (@instOfNatBaseLit (nat_lit 7)))))))))))
-          (Exp.val (Val.lit (@OfNat.ofNat BaseLit (nat_lit 8) (@instOfNatBaseLit (nat_lit 8))))))
-        (Exp.binop BinOp.xor (Exp.val (Val.lit (@OfNat.ofNat BaseLit (nat_lit 9) (@instOfNatBaseLit (nat_lit 9)))))
+                      (@ProgramLogic.ToVal.ofVal Exp Val instToVal
+                        (Val.lit ↑(@OfNat.ofNat Int (nat_lit 6) (@instOfNat (nat_lit 6)))))
+                      (@ProgramLogic.ToVal.ofVal Exp Val instToVal
+                        (Val.lit ↑(@OfNat.ofNat Int (nat_lit 7) (@instOfNat (nat_lit 7)))))))))))
+          (@ProgramLogic.ToVal.ofVal Exp Val instToVal
+            (Val.lit ↑(@OfNat.ofNat Int (nat_lit 8) (@instOfNat (nat_lit 8))))))
+        (Exp.binop BinOp.xor
+          (@ProgramLogic.ToVal.ofVal Exp Val instToVal
+            (Val.lit ↑(@OfNat.ofNat Int (nat_lit 9) (@instOfNat (nat_lit 9)))))
           (Exp.binop BinOp.shiftl
-            (Exp.val (Val.lit (@OfNat.ofNat BaseLit (nat_lit 10) (@instOfNatBaseLit (nat_lit 10)))))
+            (@ProgramLogic.ToVal.ofVal Exp Val instToVal
+              (Val.lit ↑(@OfNat.ofNat Int (nat_lit 10) (@instOfNat (nat_lit 10)))))
             (Exp.binop BinOp.shiftr
-              (Exp.val (Val.lit (@OfNat.ofNat BaseLit (nat_lit 11) (@instOfNatBaseLit (nat_lit 11)))))
-              (Exp.val (Val.lit (@OfNat.ofNat BaseLit (nat_lit 12) (@instOfNatBaseLit (nat_lit 12)))))))))
-      (Exp.binop BinOp.le (Exp.val (Val.lit (@OfNat.ofNat BaseLit (nat_lit 13) (@instOfNatBaseLit (nat_lit 13)))))
-        (Exp.binop BinOp.lt (Exp.val (Val.lit (@OfNat.ofNat BaseLit (nat_lit 14) (@instOfNatBaseLit (nat_lit 14)))))
-          (Exp.binop BinOp.eq (Exp.val (Val.lit (@OfNat.ofNat BaseLit (nat_lit 15) (@instOfNatBaseLit (nat_lit 15)))))
+              (@ProgramLogic.ToVal.ofVal Exp Val instToVal
+                (Val.lit ↑(@OfNat.ofNat Int (nat_lit 11) (@instOfNat (nat_lit 11)))))
+              (@ProgramLogic.ToVal.ofVal Exp Val instToVal
+                (Val.lit ↑(@OfNat.ofNat Int (nat_lit 12) (@instOfNat (nat_lit 12)))))))))
+      (Exp.binop BinOp.le
+        (@ProgramLogic.ToVal.ofVal Exp Val instToVal
+          (Val.lit ↑(@OfNat.ofNat Int (nat_lit 13) (@instOfNat (nat_lit 13)))))
+        (Exp.binop BinOp.lt
+          (@ProgramLogic.ToVal.ofVal Exp Val instToVal
+            (Val.lit ↑(@OfNat.ofNat Int (nat_lit 14) (@instOfNat (nat_lit 14)))))
+          (Exp.binop BinOp.eq
+            (@ProgramLogic.ToVal.ofVal Exp Val instToVal
+              (Val.lit ↑(@OfNat.ofNat Int (nat_lit 15) (@instOfNat (nat_lit 15)))))
             (Exp.binop BinOp.plus
-              (Exp.val (Val.lit (@OfNat.ofNat BaseLit (nat_lit 16) (@instOfNatBaseLit (nat_lit 16)))))
+              (@ProgramLogic.ToVal.ofVal Exp Val instToVal
+                (Val.lit ↑(@OfNat.ofNat Int (nat_lit 16) (@instOfNat (nat_lit 16)))))
               (Exp.binop BinOp.plus
                 (Exp.unop UnOp.minus
-                  (Exp.val (Val.lit (@OfNat.ofNat BaseLit (nat_lit 17) (@instOfNatBaseLit (nat_lit 17))))))
+                  (@ProgramLogic.ToVal.ofVal Exp Val instToVal
+                    (Val.lit ↑(@OfNat.ofNat Int (nat_lit 17) (@instOfNat (nat_lit 17))))))
                 (Exp.unop UnOp.neg
-                  (Exp.val (Val.lit (@OfNat.ofNat BaseLit (nat_lit 18) (@instOfNatBaseLit (nat_lit 18))))))))))))) : Exp
+                  (@ProgramLogic.ToVal.ofVal Exp Val instToVal
+                    (Val.lit ↑(@OfNat.ofNat Int (nat_lit 18) (@instOfNat (nat_lit 18))))))))))))) : Exp
 -/
 #guard_msgs in
 set_option pp.explicit true in
-#check hl(λ x y, #1 + #2 +ₗ #3 - #4 * #5 / #6 % #7 & #8 | #9 ^ #10 <<< #11 >>> #12 <= #13 ≤ #14 < #15 = #16 + (-#17) + (~#18))
+#check hl(λ x y, #1 + #2 +ₗ #3 - #4 * #5 / #6 % #7 &&& #8 ||| #9 ^^^ #10 <<< #11 >>> #12 <= #13 ≤ #14 < #15 = #16 + (-#17) + (~#18))
 
 /--
 info: Exp.binop BinOp.shiftl (Exp.var "x").load
-  (Exp.val (Val.lit (@OfNat.ofNat BaseLit (nat_lit 1) (@instOfNatBaseLit (nat_lit 1))))) : Exp
+  (@ProgramLogic.ToVal.ofVal Exp Val instToVal (Val.lit ↑(@OfNat.ofNat Int (nat_lit 1) (@instOfNat (nat_lit 1))))) : Exp
 -/
 #guard_msgs in
 set_option pp.explicit true in
@@ -150,10 +193,11 @@ set_option pp.explicit true in
 #guard_msgs in
 #check hl(if #1 then #2 else #3)
 
-/--
-info: hl(if if a then b else #(BaseLit.bool false) then #(BaseLit.bool true) else
-    if c then d else #(BaseLit.bool false)) : Exp
--/
+/-- info: hl(#1) : Exp -/
+#guard_msgs in
+#check hl(#1)
+
+/-- info: hl(if if a then b else #false then #true else if c then d else #false) : Exp -/
 #guard_msgs in
 #check hl(a && b || c && d)
 
@@ -162,22 +206,23 @@ info: hl(if if a then b else #(BaseLit.bool false) then #(BaseLit.bool true) els
 #check hl((#1, #2, #3))
 
 /--
-info: (Exp.val (Val.lit (@OfNat.ofNat BaseLit (nat_lit 1) (@instOfNatBaseLit (nat_lit 1))))).pair
-  ((Exp.val (Val.lit (@OfNat.ofNat BaseLit (nat_lit 2) (@instOfNatBaseLit (nat_lit 2))))).pair
-    (Exp.val (Val.lit (@OfNat.ofNat BaseLit (nat_lit 3) (@instOfNatBaseLit (nat_lit 3)))))) : Exp
+info: (@ProgramLogic.ToVal.ofVal Exp Val instToVal (Val.lit ↑(@OfNat.ofNat Int (nat_lit 1) (@instOfNat (nat_lit 1))))).pair
+  ((@ProgramLogic.ToVal.ofVal Exp Val instToVal (Val.lit ↑(@OfNat.ofNat Int (nat_lit 2) (@instOfNat (nat_lit 2))))).pair
+    (@ProgramLogic.ToVal.ofVal Exp Val instToVal
+      (Val.lit ↑(@OfNat.ofNat Int (nat_lit 3) (@instOfNat (nat_lit 3)))))) : Exp
 -/
 #guard_msgs in
 set_option pp.explicit true in
 #check hl((#1, #2, #3))
 
-/-- info: hl_val((#1, #BaseLit.unit, #(BaseLit.bool true), #(BaseLit.int (-1)))) : Val -/
+/-- info: hl_val((#1, #(), #true, #(-1))) : Val -/
 #guard_msgs in
-#check hl_val((#1, #(), #true, #(.int (-1))))
+#check hl_val((#1, #(), #true, #(-1 : Int)))
 
 /--
-info: (Val.lit (@OfNat.ofNat BaseLit (nat_lit 1) (@instOfNatBaseLit (nat_lit 1)))).pair
-  ((Val.lit (@OfNat.ofNat BaseLit (nat_lit 2) (@instOfNatBaseLit (nat_lit 2)))).pair
-    (Val.lit (@OfNat.ofNat BaseLit (nat_lit 3) (@instOfNatBaseLit (nat_lit 3))))) : Val
+info: (Val.lit ↑(@OfNat.ofNat Int (nat_lit 1) (@instOfNat (nat_lit 1)))).pair
+  ((Val.lit ↑(@OfNat.ofNat Int (nat_lit 2) (@instOfNat (nat_lit 2)))).pair
+    (Val.lit ↑(@OfNat.ofNat Int (nat_lit 3) (@instOfNat (nat_lit 3))))) : Val
 -/
 #guard_msgs in
 set_option pp.explicit true in
@@ -195,11 +240,11 @@ set_option pp.explicit true in
 #guard_msgs in
 #check hl(match injl(injr(#1)) with | injr(_) => #1 | injl(y) => #2)
 
-/-- info: hl(match injr(injl(#BaseLit.unit)) with | injl(_) => #2 | injr(_) => #1) : Exp -/
+/-- info: hl(match injr(injl(#())) with | injl(_) => #2 | injr(_) => #1) : Exp -/
 #guard_msgs in
 #check hl(match some(none()) with | some(_) => #1 | none() => #2)
 
-/-- info: hl(match injr(injl(#BaseLit.unit)) with | injl(_) => #1 | injr(x) => #2) : Exp -/
+/-- info: hl(match injr(injl(#())) with | injl(_) => #1 | injr(x) => #2) : Exp -/
 #guard_msgs in
 #check hl(match some(none()) with | none() => #1 | some(x) => #2)
 
@@ -207,7 +252,7 @@ set_option pp.explicit true in
 #guard_msgs in
 #check hl_val(injl(injr(#1)))
 
-/-- info: hl_val(injr(injl(#BaseLit.unit))) : Val -/
+/-- info: hl_val(injr(injl(#()))) : Val -/
 #guard_msgs in
 #check hl_val(some(none()))
 
@@ -228,29 +273,32 @@ info: (Exp.rec_ Binder.anon (Binder.named "x")
                   ((Exp.rec_ Binder.anon Binder.anon
                         ((Exp.rec_ Binder.anon Binder.anon (Exp.var "x").free).app
                           (Exp.binop BinOp.eq (Exp.var "x").load
-                              (Exp.val
-                                (Val.lit
-                                  (@OfNat.ofNat BaseLit (nat_lit 0) (@instOfNatBaseLit (nat_lit 0)))))).assert)).app
+                              (@ProgramLogic.ToVal.ofVal Exp Val instToVal
+                                (Val.lit ↑(@OfNat.ofNat Int (nat_lit 0) (@instOfNat (nat_lit 0)))))).assert)).app
                     ((Exp.rec_ Binder.anon Binder.anon
                             ((Exp.rec_ Binder.anon Binder.anon
                                   ((Exp.var "x").faa
-                                    (Exp.val
-                                      (Val.lit
-                                        (@OfNat.ofNat BaseLit (nat_lit 4) (@instOfNatBaseLit (nat_lit 4))))))).app
+                                    (@ProgramLogic.ToVal.ofVal Exp Val instToVal
+                                      (Val.lit ↑(@OfNat.ofNat Int (nat_lit 4) (@instOfNat (nat_lit 4))))))).app
                               ((Exp.var "x").xchg
-                                (Exp.val
-                                  (Val.lit (@OfNat.ofNat BaseLit (nat_lit 2) (@instOfNatBaseLit (nat_lit 2)))))))).app
+                                (@ProgramLogic.ToVal.ofVal Exp Val instToVal
+                                  (Val.lit ↑(@OfNat.ofNat Int (nat_lit 2) (@instOfNat (nat_lit 2)))))))).app
                         ((Exp.var "x").cmpXchg
-                          (Exp.val (Val.lit (@OfNat.ofNat BaseLit (nat_lit 1) (@instOfNatBaseLit (nat_lit 1)))))
-                          (Exp.val
-                            (Val.lit (@OfNat.ofNat BaseLit (nat_lit 2) (@instOfNatBaseLit (nat_lit 2))))))).fork)).app
+                          (@ProgramLogic.ToVal.ofVal Exp Val instToVal
+                            (Val.lit ↑(@OfNat.ofNat Int (nat_lit 1) (@instOfNat (nat_lit 1)))))
+                          (@ProgramLogic.ToVal.ofVal Exp Val instToVal
+                            (Val.lit ↑(@OfNat.ofNat Int (nat_lit 2) (@instOfNat (nat_lit 2))))))).fork)).app
               ((Exp.var "x").store
                 (Exp.binop BinOp.plus (Exp.var "x").load
-                  (Exp.val (Val.lit (@OfNat.ofNat BaseLit (nat_lit 1) (@instOfNatBaseLit (nat_lit 1))))))))).app
+                  (@ProgramLogic.ToVal.ofVal Exp Val instToVal
+                    (Val.lit ↑(@OfNat.ofNat Int (nat_lit 1) (@instOfNat (nat_lit 1))))))))).app
         ((Exp.var "x").load.allocN
-          (Exp.val (Val.lit (@OfNat.ofNat BaseLit (nat_lit 0) (@instOfNatBaseLit (nat_lit 0)))))))).app
-  ((Exp.val (Val.lit (@OfNat.ofNat BaseLit (nat_lit 1) (@instOfNatBaseLit (nat_lit 1))))).allocN
-    (Exp.val (Val.lit (@OfNat.ofNat BaseLit (nat_lit 0) (@instOfNatBaseLit (nat_lit 0)))))) : Exp
+          (@ProgramLogic.ToVal.ofVal Exp Val instToVal
+            (Val.lit ↑(@OfNat.ofNat Int (nat_lit 0) (@instOfNat (nat_lit 0)))))))).app
+  ((@ProgramLogic.ToVal.ofVal Exp Val instToVal
+        (Val.lit ↑(@OfNat.ofNat Int (nat_lit 1) (@instOfNat (nat_lit 1))))).allocN
+    (@ProgramLogic.ToVal.ofVal Exp Val instToVal
+      (Val.lit ↑(@OfNat.ofNat Int (nat_lit 0) (@instOfNat (nat_lit 0)))))) : Exp
 -/
 #guard_msgs in
 set_option pp.explicit true in
